

Unit - 3: Fourier Transform

Fourier Integral.

$$F(x) = \int_0^{\infty} (A(\lambda) \cos \lambda x + B(\lambda) \sin \lambda x) d\lambda$$

$$A(\lambda) = \frac{1}{\pi} \int_{-\infty}^{\infty} F(t) \cos \lambda t dt$$

$$B(\lambda) = \frac{1}{\pi} \int_{-\infty}^{\infty} F(t) \sin \lambda t dt$$

Fourier Cosine Integral

$$F(x) = \int_0^{\infty} A(\lambda) \cos \lambda x d\lambda$$

$$A(\lambda) = \frac{2}{\pi} \int_0^{\infty} F(x) \cos \lambda x dx$$

Fourier Sine Integral

$$F(x) = \int_0^{\infty} B(\lambda) \sin \lambda x d\lambda$$

$$B(\lambda) = \frac{2}{\pi} \int_0^{\infty} F(x) \sin \lambda x dx$$

1. Express the function $F(x) = 1$ For $|x| < 1$
 $= 0$ $|x| > 1$
as a Fourier Integral.

→ Solⁿ. we know,

$$F(x) = \int_0^{\infty} (A(\lambda) \cos \lambda x + B(\lambda) \sin \lambda x) d\lambda \quad \text{--- (A)}$$

$$A(\lambda) = \frac{1}{\pi} \int_{-\infty}^{\infty} F(x) \cos \lambda x dx$$

$$A(\lambda) = \frac{1}{\pi} \left[\int_{-1}^1 F(x) \cos \lambda x dx + \int_1^{\infty} F(x) \cos \lambda x dx \right]$$

$$= \frac{1}{\pi} \int_{-1}^1 1 \cos \lambda x dx + 0$$

$$= \frac{1}{\pi} \left[\frac{\sin \lambda x}{\lambda} \right]_{-1}^1$$

$$= \frac{1}{\pi \lambda} [\sin \lambda - \sin(-\lambda)]$$

$$= \frac{1}{\pi \lambda} [\sin \lambda + \sin \lambda]$$

$$= \frac{2 \sin \lambda}{\pi \lambda} \quad \text{--- (B)}$$

$$B(\lambda) = \frac{1}{\pi} \int_{-\infty}^{\infty} f(x) \sin \lambda x \, dx$$

$$= \frac{1}{\pi} \left[\int_{-1}^1 f(x) \sin \lambda x \, dx + \int_1^{\infty} f(x) \sin \lambda x \, dx \right]$$

$$= \frac{1}{\pi} \int_{-1}^1 1 \cdot \sin \lambda x \, dx + 0$$

$$= \frac{1}{\pi} \left[\frac{-\cos \lambda x}{\lambda} \right]_{-1}^1$$

$$= \frac{-1}{\pi \lambda} [\cos \lambda - \cos(-\lambda)]$$

$$B = \frac{-1}{\pi \lambda} [\cos \lambda - \cos \lambda]$$

$$B(\lambda) = 0 \quad \text{--- (C)}$$

From eqⁿ A, B & C

$$f(x) = \int_0^{\infty} \left(\frac{2 \sin \lambda \cos \lambda x}{\pi \lambda} + 0 \sin \lambda x \right) d\lambda$$

$$f(x) = \frac{2}{\pi} \int_0^{\infty} \frac{\sin \lambda \cos \lambda x}{\lambda} d\lambda$$

put $x = 0$

$$f(0) = \frac{2}{\pi} \int_0^{\infty} \frac{\sin \lambda \cos 0}{\lambda} d\lambda$$

$$1 = \frac{2}{\pi} \int_0^{\infty} \frac{\sin \lambda}{\lambda} d\lambda$$

$$\Rightarrow \int_0^{\infty} \frac{\sin \lambda}{\lambda} d\lambda = \frac{\pi}{2}$$

$$\therefore \boxed{\int_0^{\infty} \frac{\sin x}{x} dx = \frac{\pi}{2}}$$

2. Show that $\int_0^{\infty} \frac{\omega \sin x \omega}{1 + \omega^2} d\omega = \frac{\pi}{2} e^{-x}$ as Fourier sine transform.

$$F(x) = \int_0^{\infty} B(\lambda) \sin \lambda x d\lambda$$

$$B(\lambda) = \frac{2}{\pi} \int_0^{\infty} F(x) \sin \lambda x dx$$

$$B(\lambda) = \frac{2}{\pi} \int_0^{\infty} e^{-x} \sin \lambda x dx$$

$$\text{Use } \int e^{ax} \sin bx dx = \frac{e^a}{a^2 + b^2} [a \sin bx - b \cos bx]$$

$$a = -1, b = \lambda$$

$$B(\lambda) = \frac{2}{\pi} \left[\frac{e^{-x}}{(-1)^2 + \lambda^2} (-\sin \lambda x - \lambda \cos \lambda x) \right]_0^{\infty}$$

$$= \frac{2}{\pi} \left[0 - \frac{e^0}{1+\lambda^2} (-\sin 0 - \lambda \cos 0) \right]$$

$$= \frac{2}{\pi} \left[\frac{\lambda}{1+\lambda^2} \right]$$

$$= \frac{2\lambda}{\pi(1+\lambda^2)}$$

$$F(x) = e^{-x} = \int_0^{\infty} \frac{2\lambda}{\pi(1+\lambda^2)} \sin \lambda x \, d\lambda$$

$$e^{-x} = \frac{2}{\pi} \int_0^{\infty} \frac{\lambda \sin \lambda x}{1+\lambda^2} \, d\lambda$$

λ is replace by ω

$$\boxed{\frac{\pi}{2} e^{-x} = \int_0^{\infty} \frac{\omega \sin \omega x}{1+\omega^2} \, d\omega}$$

3. Using Cosine Fourier transform Show that

$$\int_0^{\infty} \frac{\cos x \omega}{1+\omega^2} \, d\omega = \frac{\pi}{2} e^{-x}$$

$$F(x) = \int_0^{\infty} A(\lambda) \cos \lambda x \, d\lambda \quad \text{--- (A)}$$

$$A(\lambda) = \frac{2}{\pi} \int_0^{\infty} F(x) \cos \lambda x \, dx$$

$$= \frac{2}{\pi} \int_0^{\infty} e^{-x} \cos \lambda x \, dx$$

Use $\int e^{ax} \cos bx \, dx = \frac{e^{ax}}{a^2 + b^2} (a \cos bx + b \sin bx)$

$$a = -1, \quad b = \lambda$$

$$BA(\lambda) = \frac{2}{\pi} \left[\frac{e^{-x}}{(-1)^2 + \lambda^2} (-\cos \lambda x + \lambda \sin \lambda x) \right]_0^{\infty}$$

$$= \frac{2}{\pi} \left[0 - \frac{e^0}{1 + \lambda^2} (-\cos 0 + \lambda \sin 0) \right]$$

$$= \frac{2}{\pi} \left[\frac{1}{1 + \lambda^2} \right]$$

$$A(\lambda) = \frac{2}{\pi(1 + \lambda^2)}$$

eqⁿ (A) becomes

$$F(x) = e^{-x} = \int_0^{\infty} \frac{2}{\pi(1 + \lambda^2)} \cos \lambda x \, d\lambda$$

$$e^{-x} = \frac{2}{\pi} \int_0^{\infty} \frac{\cos \lambda x}{(1 + \lambda^2)} \, d\lambda$$

λ is replaced by u

$$\boxed{\frac{\pi}{2} e^{-x} = \int_0^{\infty} \frac{\cos ux}{1 + u^2} \, du}$$

Fourier Transform

$$F(s) = \int_{-\infty}^{\infty} F(t) e^{ist} dt$$

Inverse Fourier Transform

$$F(x) = \frac{1}{2\pi} \int_{-\infty}^{\infty} F(s) e^{-isx} ds$$

* Examples

1. Find the Fourier transform for

$$F(x) = 1 - x^2 \quad |x| \leq 1 \quad \text{and hence evaluate} \\ = 0 \quad |x| > 1$$

$$\int_0^{\infty} \left(\frac{x \cos x - \sin x}{x^3} \right) \cos \frac{x}{2} dx$$



We have

$$F(x) = 1 - x^2 \quad |x| \leq 1 \Rightarrow -1 \leq x \leq 1 \\ = 0 \quad |x| > 1 \Rightarrow 1 < x < \infty$$

By using Fourier Transform

$$F(s) = \int_{-\infty}^{\infty} F(x) e^{isx} dx$$

$$= \int_{-1}^1 F(x) (\cos sx + i \sin sx) dx + \int_1^{\infty} F(x) (\cos sx + i \sin sx) dx$$

$$= \int_{-1}^1 (1 - x^2) (\cos sx + i \sin sx) dx + 0$$

$$F(s) = \int_{-1}^1 (1-x^2) \cos sx \, dx + \int_{-1}^1 (1-x^2) i \sin sx \, dx \quad \text{--- (A)}$$

Consider

$$F_1(x) = (1-x^2) \cos sx$$

$$F_1(-x) = (1-(-x)^2) \cos s(-x)$$

$$= (1-x^2) \cos sx = F_1(x)$$

$$\Rightarrow F_1(-x) = F_1(x)$$

$\Rightarrow F_1(x)$ is even function

$$F_2(x) = (1-x^2) \sin sx$$

$$F_2(-x) = (1-(-x)^2) \sin s(-x)$$

$$= (1-x^2) (-\sin sx)$$

$$\therefore F_2(-x) = -F_2(x)$$

$F_2(x)$ is odd

Eqⁿ (A) becomes

$$F(s) = \int_{-1}^1 (1-x^2) \cos sx \, dx + \int_{-1}^1 (1-x^2) i \sin sx \, dx$$

\uparrow even function \uparrow odd function

$$= 2 \int_0^1 (1-x^2) \cos sx \, dx + 0$$

$$= 2 \left[(1-x^2) \frac{\sin sx}{s} - (0-2x) \frac{(-\cos sx)}{s \times s} + \frac{(-2)(-\sin sx)}{s^2 \times s} \right]_0^1$$

$$= 2 \left[0 - 2 \times 1 \frac{\cos s}{s^2} + \frac{2 \sin s}{s^3} - 0 - 0 - 0 \right]$$

$$= 2 \left[-\frac{2 \cos s}{s^2} + \frac{2 \sin s}{s^3} \right]$$

$$= -4 \left[\frac{s \cos s - \sin s}{s^3} \right] \rightarrow \textcircled{B}$$

By using Inverse Fourier Transform

$$F(x) = \frac{1}{2\pi} \int_{-\infty}^{\infty} F(s) e^{-isx} ds$$

$$= \frac{1}{2\pi} \int_{-\infty}^{\infty} \frac{-4(s \cos s - \sin s)}{s^3} (\cos sx - i \sin sx) ds$$

$$= \frac{2(-4)}{2\pi} \int_0^{\infty} \left(\frac{s \cos s - \sin s}{s^3} \right) \cos sx ds$$

Here $\cos sx$ even Function
 $\sin sx$ odd Function

$$1 - x^2 = F(x) = -\frac{4}{\pi} \int_0^{\infty} \left(\frac{s \cos s - \sin s}{s^3} \right) \cos sx ds$$

$$\text{put } s = x \text{ \& } x = 1/2$$

$$1 - (1/2)^2 = -\frac{4}{\pi} \int_0^{\infty} \left(\frac{x \cos x - \sin x}{x^3} \right) \cos \frac{x}{2} dx$$

$$1 - \frac{1}{4} = -\frac{4}{\pi} \int_0^{\infty} \left(\frac{x \cos x - \sin x}{x^3} \right) \cos \frac{x}{2} dx$$

$$\frac{3}{4} = -\frac{4}{\pi} \int_0^{\infty} \left(\frac{x \cos x - \sin x}{x^3} \right) \cos \frac{x}{2} dx$$

$$\Rightarrow \int_0^{\infty} \left(\frac{x \cos x - \sin x}{x^3} \right) \cos \frac{x}{2} dx = \frac{3}{4} \times \left(-\frac{\pi}{4} \right)$$

$$\boxed{\int_0^{\infty} \left(\frac{x \cos x - \sin x}{x^3} \right) \cos \frac{x}{2} dx = -\frac{3\pi}{16}}$$

2. Find Fourier sine transform of $\frac{e^{-ax}}{x}$

→ we have $F(x) = \frac{e^{-ax}}{x}$

Fourier transform of $F(x)$ is

$$F_s(s) = \int_0^{\infty} F(x) \sin sx \, dx$$

$$F_s(s) = \int_0^{\infty} \frac{e^{-ax}}{x} \sin sx \, dx = I \text{ (say)} \quad \text{--- (I)}$$

diff w.r.t. s

$$\frac{dI}{ds} = \int_0^{\infty} \frac{e^{-ax}}{x} \cos sx \times x \, dx$$

$$\frac{dI}{ds} = \int_0^{\infty} e^{-ax} \cos sx \, dx$$

use $\int_0^{\infty} e^{ax} \cos bx \, dx = \frac{e^{ax}}{a^2 + b^2} (a \cos bx - b \sin bx)$

$$a = -a, \quad b = s$$

$$= \left[\frac{e^{-ax}}{(-a)^2 + s^2} [-a \cos sx - s \sin sx] \right]_0^\infty$$

$$= 0 - \left(\frac{e^0}{a^2 + s^2} (-a \cos 0 - s \sin 0) \right)$$

$$= \frac{a}{a^2 + s^2}$$

$$\therefore \frac{dI}{ds} = \frac{a}{a^2 + s^2}$$

$$dI = \frac{a}{a^2 + s^2} ds$$

on integration

$$\int dI = \int \frac{a}{a^2 + s^2} ds$$

$$I = a \times \frac{1}{a} \tan^{-1} \left(\frac{s}{a} \right) + c$$

$$I = \tan^{-1} \left(\frac{s}{a} \right) + c \quad \text{--- (A)}$$

Put $s=0$ in eqⁿ (I)

$$I = F(s) = 0$$

$$\therefore I = 0$$

Put this value in eqⁿ (A)

$$0 = \tan^{-1}(0) + C$$

$$0 = 0 + C$$

$$\Rightarrow \boxed{C=0}$$

eqⁿ (A) becomes

$$I = F(s) = \int_0^{\infty} \frac{e^{-ax}}{x} \sin sx \, dx$$

$$= \tan^{-1}\left(\frac{s}{a}\right) + C$$

$$\therefore \boxed{I = \tan^{-1}\left(\frac{s}{a}\right)}$$

Fourier Transform

$$F(s) = \int_{-\infty}^{\infty} F(t) e^{ist} dt$$

is called Fourier transform

$$F(x) = \frac{1}{2\pi} \int_{-\infty}^{\infty} F(s) e^{isx} dx$$

is called inverse Fourier transform

Fourier Sine and cosine transform

$$F_c(s) = \int_0^{\infty} F(x) \cos sx dx$$

is called Fourier cosine transform

$$F(x) = \frac{2}{\pi} \int_0^{\infty} F_c(s) \cos sx ds$$

is called Inverse Fourier cosine Transform

$$F_s(s) = \int_0^{\infty} F(x) \sin sx dx$$

is called Fourier sine transform

$$F(x) = \frac{2}{\pi} \int_0^{\infty} F_s(s) \sin sx ds$$

is called inverse Fourier sine transform

1. Find the Fourier sine transform of

$e^{-|x|}$ and hence show that

$$\int_0^{\infty} \frac{x \sin mx}{1+x^2} dx = \frac{\pi e^{-m}}{2} \quad m > 0$$

→ Let $F(x) = e^{-|x|} = e^{-x}$

By using Fourier Sine transform formula.

$$F_s(s) = \int_0^{\infty} F(x) \sin sx dx$$

$$F_s(s) = \int_0^{\infty} e^{-x} \sin sx dx$$

use $\int e^{ax} \sin bx dx = \frac{e^{ax}}{a^2+b^2} [a \sin bx - b \cos bx]$

$a = -1, b = s$

$$F_s(s) = \left[\frac{e^{-x}}{(-1)^2 + s^2} (-\sin sx - s \cos sx) \right]_0^{\infty}$$

$$= 0 - \left[\frac{e^0}{1+s^2} (-\sin 0 - s \cos 0) \right]$$

$$= - \left[\frac{1}{1+s^2} (-0 - s) \right]$$

$$F_s(s) = \frac{s}{1+s^2}$$

By using Inverse Fourier Sine Transform Formula

$$F(x) = \frac{2}{\pi} \int_0^{\infty} F_s(s) \sin sx \, ds$$

$$F(x) = \frac{2}{\pi} \int_0^{\infty} \frac{s}{1+s^2} \sin sx \, ds$$

Put $s=x$ & $x=m$ we get

$$F(x) = e^{-m} = \frac{2}{\pi} \int_0^{\infty} \frac{x \sin xm}{1+x^2} \, dx$$

$$\boxed{\int_0^{\infty} \frac{x \sin mx}{1+x^2} \, dx = \frac{\pi}{2} e^{-m}}$$

2. Find the Fourier Cosine transform of $F(x) = \frac{1}{1+x^2}$ and hence derive the

Fourier sine transform of $\phi(x) = \frac{x}{1+x^2}$

→ Solⁿ, we have $F(x) = \frac{1}{1+x^2}$

$$F_c(s) = \int_0^{\infty} F(x) \cos sx \, dx$$

$$F_c(s) = \int_0^{\infty} \frac{1}{1+x^2} \cos x \, dx$$

$$I = \int_0^{\infty} \left(\frac{\cos sx}{1+x^2} \right) dx \quad \text{--- (1)}$$

diff w.r.t. s

$$\frac{dI}{ds} = \int_0^{\infty} \left(\frac{1}{1+x^2} \right) (-\sin sx) x \, dx \quad \text{--- (*)}$$

$$= - \int_0^{\infty} \frac{x}{(1+x^2)} \sin sx \, dx$$

$$= - \int_0^{\infty} \frac{x^2 \sin sx}{x(1+x^2)} \, dx$$

$$= - \int_0^{\infty} \frac{(1+x^2-1) \sin sx}{x(1+x^2)} \, dx$$

$$= - \int_0^{\infty} \frac{1+x^2}{x(1+x^2)} \sin sx \, dx + \int_0^{\infty} \frac{1}{x(1+x^2)} \sin sx \, dx$$

$$= - \int_0^{\infty} \frac{\sin sx}{x} \, dx + \int_0^{\infty} \frac{\sin sx}{x(1+x^2)} \, dx$$

$$\frac{dI}{ds} = -\frac{\pi}{2} + \int_0^{\infty} \frac{\sin sx}{x(1+x^2)} \, dx \quad \text{--- (2)}$$

Diff w.r.t. s

$$\frac{d^2 I}{ds^2} = 0 + \int_0^{\infty} \frac{\cos sx \times x}{x(1+x^2)} \, dx$$

$$\frac{d^2 I}{ds^2} = I$$

$$\frac{d^2 I}{ds^2} - I = 0$$

A.E eqⁿ

$$m^2 - 1 = 0$$

$$(m-1)(m+1) = 0$$

$$m = 1, m = -1$$

$$C.F = I = C_1 e^{m_1 s} + C_2 e^{m_2 s}$$

$$I = C_1 e^s + C_2 e^{-s} \text{ — (III)}$$

Diff. w.r.t. s

$$\frac{dI}{ds} = C_1 e^s \times 1 + C_2 e^{-s} \times (-1)$$

$$\frac{dI}{ds} = C_1 e^s - C_2 e^{-s} \text{ — (IV)}$$

Put $s=0$ in eqⁿ (I)

$$F(s) = \int_0^\infty \frac{1}{1+x^2} \cos 0 \, dx$$

$$F(s) = \int_0^\infty \frac{1}{1+x^2} \, dx$$

$$= (\tan^{-1} x)_0^\infty$$

$$I = \tan^{-1} \infty - \tan^{-1}(0)$$

$$I = \frac{\pi}{2} - 0$$

$$\boxed{I = \frac{\pi}{2}} \longrightarrow \textcircled{a}$$

Put $s=0$ in eqⁿ \textcircled{II}

$$\frac{dI}{ds} = -\frac{\pi}{2} + \int_0^{\infty} \frac{\sin sx}{x(1+x^2)} dx$$

$$\frac{dI}{ds} = -\frac{\pi}{2} + \int_0^{\infty} \frac{\sin 0}{x(1+x^2)} dx$$

$$\boxed{\frac{dI}{ds} = -\frac{\pi}{2}} \text{ --- } \textcircled{b}$$

Put $s=0$ in eqⁿ \textcircled{III}

$$\frac{\pi}{2} = C_1 e^0 + C_2 e^0 \quad \text{--- From eqⁿ } \textcircled{a}$$

$$\frac{\pi}{2} = C_1 + C_2 \quad \text{--- } \textcircled{A}$$

Put $s=0$ in eqⁿ \textcircled{IV} and From eqⁿ \textcircled{b}

$$-\frac{\pi}{2} = C_1 e^0 - C_2 e^0$$

$$-\frac{\pi}{2} = c_1 - c_2 \quad \text{--- (B)}$$

$$c_1 + c_2 = \pi/2$$

$$c_1 - c_2 = -\pi/2$$

$$2c_1 + 0 = 0$$

$$c_1 = 0$$

$$c_2 = \frac{\pi}{2}$$

$$I = \text{C.F} = c_1 e^s + c_2 e^{-s}$$

$$= 0 e^s + \frac{\pi}{2} e^{-s}$$

$$\therefore I = \frac{\pi}{2} e^{-s}$$

$$I = F(s) = \int_0^{\infty} \frac{1}{(1+x^2)} \cos sx \, dx = \frac{\pi}{2} e^{-s}$$

$$I = \frac{\pi}{2} e^{-s}$$

diff. w.r.t. s

$$\frac{dI}{ds} = \frac{\pi}{2} e^{-s} \times -1$$

$$= -\frac{\pi}{2} e^{-s}$$

From eqⁿ (*)

$$\int_0^{\infty} \frac{-x \sin sx}{(1+x^2)} dx = -\frac{\pi}{2} e^{-s}$$

$$= - \int_0^{\infty} \frac{x}{1+x^2} \sin sx dx$$

$$\Rightarrow -F_s(s) = -\frac{\pi}{2} e^{-s}$$

$$F_s(s) = \int_0^{\infty} \frac{x}{1+x^2} \sin sx dx = \frac{\pi}{2} e^{-s}$$

Finite Fourier Transform

• Finite Fourier sine transform :-

$$F_s(n) = \int_0^c f(x) \sin \frac{n\pi x}{c} dx \quad \text{is called}$$

Finite Fourier Sine transform

$$f(x) = \frac{2}{c} \sum_{n=1}^{\infty} F_s(n) \sin \frac{n\pi x}{c} \quad \text{is called}$$

Inverse Finite Fourier sine transform

• Finite Fourier Cosine Transform

$$F_c(n) = \int_0^c f(x) \cos \frac{n\pi x}{c} dx \quad \text{is}$$

called Finite Fourier cosine Transform

$$f(x) = \frac{2}{c} \sum_{n=1}^{\infty} F_c(n) \frac{\cos n\pi x}{c}$$

Examples.

1. Find Fourier cosine and sine transform of $f(x) = 2x$ $0 < x < 4$

→ Solⁿ, we have

$$f(x) = 2x \quad 0 < x < 4$$

$$\Rightarrow c = 4$$

Finite Fourier cosine transform

$$F_c(n) = \int_0^c f(x) \cos \frac{n\pi x}{c} dx$$

$$F_c(n) = \int_0^4 2x \cos \frac{n\pi x}{4} dx$$

$$= 2 \int_0^4 x \cos \frac{n\pi x}{4} dx$$

Use by parts rule: $\int u v dx = u \int v dx - \int \left[\frac{du}{dx} \int v dx \right]$

$$= 2 \left[x \frac{\sin \frac{n\pi x}{4}}{\frac{n\pi}{4}} - 1 \frac{1}{n\pi/4} (-\cos \frac{n\pi x}{4}) \frac{1}{n\pi/4} \right]_0^4$$

$$= 2 \left[\frac{4x}{n\pi} \sin \frac{n\pi x}{4} + \frac{16}{n^2\pi^2} \cos \frac{n\pi x}{4} \right]_0^4$$

$$= 2 \left[\frac{4 \times 4}{n\pi} \sin \frac{4n\pi}{4} + \frac{16}{n^2\pi^2} \cos \frac{4n\pi}{4} - \left(0 + \frac{16}{n^2\pi^2} \cos 0 \right) \right]$$

$$= 2 \left[0 + \frac{16}{n^2\pi^2} (-1)^n - \frac{16}{n^2\pi^2} \times 1 \right]$$

$$= \frac{32}{n^2\pi^2} [(-1)^n - 1] = \frac{32}{n^2\pi^2} [\cos n\pi - 1]$$

$$F_s(n) = \int_0^c F(x) \frac{\sin n\pi x}{c} dx$$

$$= \int_0^4 2x \sin \frac{n\pi x}{4} dx$$

$$= 2 \int_0^4 x \sin \frac{n\pi x}{4} dx$$

$$= 2 \left[x \frac{(-\cos(n\pi x/4))}{n\pi/4} - \frac{(-\sin(n\pi x/4))}{n\pi/4 \times n\pi/4} \right]_0^4$$

$$= 2 \left[-\frac{4x}{n\pi} \cos \frac{n\pi x}{4} + \frac{16}{n^2\pi^2} \sin \frac{n\pi x}{4} \right]_0^4$$

$$= 2 \left[\frac{-4 \times 4}{n\pi} \cos \frac{4n\pi}{4} - \frac{-4 \times 0 \times \cos 0}{n\pi} \right]$$

$$= 2 \left[\frac{-16}{n\pi} \cos n\pi \right]$$

$$= \frac{-32 \cos n\pi}{n\pi}$$

Parseval's Identity:

$$1. \quad \frac{1}{2\pi} \int_{-\infty}^{\infty} F(s) G(s) ds = \int_{-\infty}^{\infty} F(x) g(x) dx$$

$$2. \quad \frac{1}{2\pi} \int_{-\infty}^{\infty} (F(s))^2 ds = \int_{-\infty}^{\infty} (F(x))^2 dx$$

$$1. \quad \frac{2}{\pi} \int_0^{\infty} F_c(s) G_c(s) ds = \int_0^{\infty} F(x) g(x) dx$$

$$2. \quad \frac{2}{\pi} \int_0^{\infty} F_s(s) G_s(s) ds = \int_0^{\infty} F(x) g(x) dx$$

$$3. \quad \frac{2}{\pi} \int_0^{\infty} (F_c(s))^2 ds = \int_0^{\infty} (F(x))^2 dx$$

$$4. \quad \frac{2}{\pi} \int_0^{\infty} (F_s(s))^2 ds = \int_0^{\infty} (F(x))^2 dx$$

* Example :

1. Evaluate $\int_0^{\infty} \frac{1}{(x^2+a^2)(x^2+b^2)} dx$

→ Solⁿ let $F(x) = e^{-ax}$ $F_c(s) = \frac{a}{a^2+s^2}$

$$g(x) = e^{-bx} \quad \mathcal{F}\{G_c(s)\} = \frac{b}{b^2+s^2}$$

By using Parseval's Identity

$$\frac{2}{\pi} \int_0^{\infty} F_c(s) G_c(s) ds = \int_0^{\infty} F(x) \cdot g(x) \cdot dx$$

$$\frac{2}{\pi} \int_0^{\infty} \left(\frac{a}{a^2+s^2} \cdot \frac{b}{b^2+s^2} \right) ds = \int_0^{\infty} (e^{-ax} \cdot e^{-bx}) dx$$

$$\frac{2ab}{\pi} \int_0^{\infty} \frac{1}{(s^2+a^2)(s^2+b^2)} ds = \int_0^{\infty} e^{-ax-bx} dx$$

$$\frac{2ab}{\pi} \int_0^{\infty} \frac{1}{(s^2+a^2)(s^2+b^2)} ds = \left[\frac{e^{-x(a+b)}}{-(a+b)} \right]_0^{\infty}$$

$$= 0 - \left(\frac{e^0}{-(a+b)} \right)$$

$$= \frac{1}{a+b}$$

$$\int_0^{\infty} \frac{1}{(s^2+a^2)(s^2+b^2)} ds = \frac{\pi}{(2ab)(a+b)}$$

$$\int_0^{\infty} \frac{1}{(x^2+a^2)(x^2+b^2)} = \frac{\pi}{(2ab)(a+b)}$$

2 Using Parseval's Identity prove that

$$\int_0^{\infty} \frac{t^2}{(1+t^2)^2} dt$$

→

Solⁿ

Let $F(x) = \frac{x}{(1+x^2)}$ then $F_s(s) = \frac{\pi}{2} e^{-s}$

By using Parseval's Identity

$$\frac{2}{\pi} \int_0^{\infty} (F_s(s))^2 ds = \int_0^{\infty} (F(x))^2 dx$$

$$\frac{2}{\pi} \int_0^{\infty} \left(\frac{\pi}{2} e^{-s} \right)^2 ds = \int_0^{\infty} \left[\frac{x}{(1+x^2)} \right]^2 dx$$

$$\frac{2}{\pi} \int_0^{\infty} \frac{\pi^2}{4} e^{-2s} ds = \int_0^{\infty} \frac{x^2}{(1+x^2)^2} dx$$

$$\frac{2}{\pi} \times \frac{\pi^2}{4} \int_0^{\infty} e^{-2s} ds = \int_0^{\infty} \frac{x^2}{(1+x^2)^2} dx$$

$$\frac{\pi}{2} \left[\frac{e^{-2s}}{-2} \right]_0^{\infty} = \int_0^{\infty} \frac{x^2}{(1+x^2)^2} dx$$

$$\frac{\pi}{2} \times \frac{-1}{2} [0 - e^0] = \int_0^{\infty} \frac{x^2}{(1+x^2)^2} dx$$

$$\frac{\pi}{4} = \int_0^{\infty} \frac{x^2}{(1+x^2)^2} dx$$

$$\therefore \boxed{\int_0^{\infty} \frac{t^2}{(1+t^2)^2} dt = \frac{\pi}{4}}$$

3. By using Parseval's Identity show that

$$\int_0^{\infty} \frac{1}{(t^2+1)^2} dt = \frac{\pi}{4}$$

→ Let $F(x) = e^{-x}$ then $F_c(s) = \frac{1}{s^2+1}$

By using Parseval's Identity

$$\frac{2}{\pi} \int_0^{\infty} (F_c(s))^2 ds = \int_0^{\infty} (F(x))^2 dx$$

$$\frac{2}{\pi} \int_0^{\infty} \left(\frac{1}{s^2+1} \right)^2 ds = \int_0^{\infty} (e^{-x})^2 dx$$

$$\frac{2}{\pi} \int_0^{\infty} \frac{1}{(s^2+1)^2} ds = \int_0^{\infty} e^{-2x} dx$$

$$\frac{2}{\pi} \int_0^{\infty} \frac{1}{(s^2+1)^2} ds = \left[\frac{e^{-2x}}{-2} \right]_0^{\infty}$$

$$\frac{2}{\pi} \int_0^{\infty} \frac{1}{(s^2+1)^2} ds = -\frac{1}{2} [0 - e^0]$$

$$\frac{2}{\pi} \int_0^{\infty} \frac{1}{(s^2+1)^2} ds = -\frac{1}{2} (0 - 1)$$

$$\int_0^{\infty} \frac{1}{(s^2+1)^2} ds = \frac{1}{2} \times \frac{\pi}{2}$$

$$\boxed{\int_0^{\infty} \frac{1}{(t^2+1)^2} dt = \frac{\pi}{4}}$$

4. By Using Parseval's Identity Show that

$$\int_0^{\infty} \frac{t^2}{(4+t^2)(9+t^2)} dt = \frac{\pi}{10}$$

→ let $F(x) = \frac{x}{4+x^2} = \frac{x}{2^2+x^2}$ then $F_s(s) = \frac{\pi}{2} e^{-2s}$

$g(x) = \frac{x}{9+x^2} = \frac{x}{3^2+x^2}$ then $G_s(s) = \frac{\pi}{2} e^{-3s}$

By Using Parseval's Identity

$$\frac{2}{\pi} \int_0^{\infty} F_s(s) \cdot G_s(s) ds = \int_0^{\infty} F(x) \cdot g(x) dx$$

$$\frac{2}{\pi} \int_0^{\infty} \left(\frac{x}{4+x^2} \cdot \frac{x}{9+x^2} \right) dx = \int_0^{\infty}$$

$$\frac{2}{\pi} \int_0^{\infty} \left(\frac{\pi}{2} e^{-2s} \cdot \frac{\pi}{2} e^{-3s} \right) ds = \int_0^{\infty} \frac{x}{(4+x^2)(9+x^2)} dx$$

$$\frac{2}{\pi} \times \frac{\pi^2}{4} \int_0^{\infty} e^{-2s-3s} ds = \int_0^{\infty} \frac{x^2}{(4+x^2)(9+x^2)} dx$$

$$\frac{\pi}{2} \left[\frac{e^{-5s}}{-5} \right]_0^{\infty} = \int_0^{\infty} \frac{x^2}{(4+x^2)(9+x^2)} dx$$

$$-\frac{\pi}{10} [0 - e^0] = \int_0^{\infty} \frac{x^2}{(4+x^2)(9+x^2)} dx$$

$$-\frac{\pi}{10} [0 - 1] = \int_0^{\infty} \frac{x^2}{(4+x^2)(9+x^2)} dx$$

$$\frac{\pi}{10} = \int_0^{\infty} \frac{x^2}{(4+x^2)(9+x^2)} dx$$

$$\Rightarrow \boxed{\int_0^{\infty} \frac{t^2}{(4+t^2)(9+t^2)} dt = \frac{\pi}{10}}$$